@prefix : <http://field33.com/ontologies/@fld33_domain/software_architecture_metric/> .
@prefix owl: <http://www.w3.org/2002/07/owl#> .
@prefix rdf: <http://www.w3.org/1999/02/22-rdf-syntax-ns#> .
@prefix xml: <http://www.w3.org/XML/1998/namespace> .
@prefix xsd: <http://www.w3.org/2001/XMLSchema#> .
@prefix rdfs: <http://www.w3.org/2000/01/rdf-schema#> .
@prefix registry: <http://field33.com/ontologies/REGISTRY/> .
@base <http://field33.com/ontologies/@fld33_domain/software_architecture_metric/> .

<http://field33.com/ontologies/@fld33_domain/software_architecture_metric/> rdf:type owl:Ontology ;
                                                                             owl:imports <http://field33.com/ontologies/@fld33/methodology/> ,
                                                                                         <http://field33.com/ontologies/@fld33/relations_0_1_0/> ;
                                                                             registry:author "Field 33 <contribution@field33.com>" ;
                                                                             registry:canonicalPrefix "software_architecture_metric" ;
                                                                             registry:category "Metric" ,
                                                                                               "Software Architecture" ,
                                                                                               "Software Development" ;
                                                                             registry:dependency "@fld33/methodology ^0.1.7" ,
                                                                                                 "@fld33/relations_0_1_0 ^0.1.10" ;
                                                                             registry:keyword "Field 33 Package" ,
                                                                                              "Metric" ,
                                                                                              "Software Architecture" ,
                                                                                              "Software Architecture Metric" ,
                                                                                              "Software Development" ;
                                                                             registry:ontologyFormatVersion "v1" ;
                                                                             registry:packageName "@fld33_domain/software_architecture_metric" ;
                                                                             registry:packageVersion "0.1.4" ;
                                                                             registry:licenseSPDX "Apache-2.0" ;
                                                                             registry:repository "https://github.com/field33/ontologies/tree/main/%40fld33_domain/software_architecture_metric" ;
                                                                             registry:shortDescription "Software architecture metric ontology"@en ;
                                                                             rdfs:comment "#Software Architecture Metric Ontology<br>This package is an internal ontology describing concepts for software architecture metrics."@en ;
                                                                             rdfs:label "Software Architecture Metric"@en .


#################################################################
#    Classes
#################################################################

###  http://field33.com/ontologies/@fld33_domain/software_architecture_metric/Adaptability
:Adaptability rdf:type owl:Class ;
              rdfs:subClassOf <http://field33.com/ontologies/@fld33/methodology/Metric> ;
              rdfs:comment "Adaptability of software system or software architecture is (1) a qualitative property of its maintainability and (2) an ability of its components to adapt their functionality, even at runtime, to behavioral and structural changes that occur either internally or externally in their operating environment and in requirements of stakeholders objectives"@en ;
              rdfs:label "Adaptability"@en .


###  http://field33.com/ontologies/@fld33_domain/software_architecture_metric/BottleneckElimination
:BottleneckElimination rdf:type owl:Class ;
                       rdfs:subClassOf <http://field33.com/ontologies/@fld33/methodology/Metric> ;
                       rdfs:label "Bottleneck Elimination"@en .


###  http://field33.com/ontologies/@fld33_domain/software_architecture_metric/CostOptimization
:CostOptimization rdf:type owl:Class ;
                  rdfs:subClassOf <http://field33.com/ontologies/@fld33/methodology/Metric> ;
                  rdfs:comment "Cost Optimization includes the ability to run systems to deliver business value at the lowest price point."@en ;
                  rdfs:label "Cost Optimization"@en ;
                  rdfs:seeAlso "https://wa.aws.amazon.com/wellarchitected/2020-07-02T19-33-23/wat.pillar.costOptimization.en.html"@en .


###  http://field33.com/ontologies/@fld33_domain/software_architecture_metric/OperationalExcellence
:OperationalExcellence rdf:type owl:Class ;
                       rdfs:subClassOf <http://field33.com/ontologies/@fld33/methodology/Metric> ;
                       rdfs:comment "Operational Excellence includes the ability to support development and run workloads effectively, gain insight into their operations, and to continuously improve supporting processes and procedures to deliver business value."@en ;
                       rdfs:label "Operational Excellence"@en ;
                       rdfs:seeAlso "https://wa.aws.amazon.com/wellarchitected/2020-07-02T19-33-23/wat.pillar.operationalExcellence.en.html"@en .


###  http://field33.com/ontologies/@fld33_domain/software_architecture_metric/PerformanceEfficiency
:PerformanceEfficiency rdf:type owl:Class ;
                       rdfs:subClassOf <http://field33.com/ontologies/@fld33/methodology/Metric> ;
                       rdfs:comment "The Performance Efficiency includes the ability to use computing resources efficiently to meet system requirements, and to maintain that efficiency as demand changes and technologies evolve."@en ;
                       rdfs:label "Performance Efficiency"@en ;
                       rdfs:seeAlso "https://wa.aws.amazon.com/wellarchitected/2020-07-02T19-33-23/wat.pillar.performance.en.html"@en .


###  http://field33.com/ontologies/@fld33_domain/software_architecture_metric/Reliability
:Reliability rdf:type owl:Class ;
             rdfs:subClassOf <http://field33.com/ontologies/@fld33/methodology/Metric> ;
             rdfs:comment "Reliability encompasses the ability of a workload to perform its intended function correctly and consistently when its expected to. This includes the ability to operate and test the workload through its total lifecycle"@en ;
             rdfs:label "Reliability"@en ;
             rdfs:seeAlso "https://wa.aws.amazon.com/wellarchitected/2020-07-02T19-33-23/wat.pillar.reliability.en.html"@en .


###  http://field33.com/ontologies/@fld33_domain/software_architecture_metric/Security
:Security rdf:type owl:Class ;
          rdfs:subClassOf <http://field33.com/ontologies/@fld33/methodology/Metric> ;
          rdfs:comment "Security encompasses the ability to protect data, systems, and assets to take advantage of cloud technologies to improve your security."@en ;
          rdfs:label "Security"@en ;
          rdfs:seeAlso "https://wa.aws.amazon.com/wellarchitected/2020-07-02T19-33-23/wat.pillar.security.en.html"@en .


###  Generated by the OWL API (version 4.5.9.2019-02-01T07:24:44Z) https://github.com/owlcs/owlapi
