@prefix : <http://field33.com/ontologies/@fld33_domain/software_team_metric/> .
@prefix owl: <http://www.w3.org/2002/07/owl#> .
@prefix rdf: <http://www.w3.org/1999/02/22-rdf-syntax-ns#> .
@prefix xml: <http://www.w3.org/XML/1998/namespace> .
@prefix xsd: <http://www.w3.org/2001/XMLSchema#> .
@prefix rdfs: <http://www.w3.org/2000/01/rdf-schema#> .
@prefix registry: <http://field33.com/ontologies/REGISTRY/> .
@base <http://field33.com/ontologies/@fld33_domain/software_team_metric/> .

<http://field33.com/ontologies/@fld33_domain/software_team_metric/> rdf:type owl:Ontology ;
                                                                     owl:imports <http://field33.com/ontologies/@fld33/methodology/> ,
                                                                                 <http://field33.com/ontologies/@fld33/relations/> ;
                                                                     registry:author "Field 33 <contribution@field33.com>" ;
                                                                     registry:canonicalPrefix "software_team_metric" ;
                                                                     registry:category "Metric" ,
                                                                                       "Organization" ,
                                                                                       "Software Development" ;
                                                                     registry:dependency "@fld33/methodology ^0.1.7" ,
                                                                                         "@fld33/relations ^0.2.2" ,
                                                                                         "@fld33_domain/software_development ^0.3.0" ;
                                                                     registry:keyword "Field 33 Package" ,
                                                                                      "Metric" ,
                                                                                      "Organization" ,
                                                                                      "Software Development" ,
                                                                                      "Software Team Metric" ;
                                                                     registry:ontologyFormatVersion "v1" ;
                                                                     registry:packageName "@fld33_domain/software_team_metric" ;
                                                                     registry:packageVersion "0.2.0" ;
                                                                     registry:licenseSPDX "Apache-2.0" ;
                                                                     registry:repository "https://github.com/field33/ontologies/tree/main/%40fld33_domain/software_team_metric" ;
                                                                     registry:shortDescription "Software team metric ontology"@en ;
                                                                     rdfs:comment "# Software Team Metric Ontology<br>This package is an internal ontology describing concepts for software team metrics."@en ;
                                                                     rdfs:label "Software Team Metric"@en .

#################################################################
#    Classes
#################################################################

###  http://field33.com/ontologies/@fld33_domain/software_team_metric/AverageWaitingTime
:AverageWaitingTime rdf:type owl:Class ;
                    rdfs:subClassOf :WaitingTime ;
                    rdfs:label "Average Waiting Time"@en .


###  http://field33.com/ontologies/@fld33_domain/software_team_metric/ChangeFailureRate
:ChangeFailureRate rdf:type owl:Class ;
                   rdfs:subClassOf <http://field33.com/ontologies/@fld33/methodology/Metric> ;
                   rdfs:comment "The change failure rate is the percentage of code changes that require hot fixes or other remediation after production. This does not measure failures caught by testing and fixed before code is deployed."@en ;
                   rdfs:label "Change Failure Rate"@en ;
                   rdfs:seeAlso "https://www.atlassian.com/devops/frameworks/devops-metrics"@en .


###  http://field33.com/ontologies/@fld33_domain/software_team_metric/ChangeLeadTime
:ChangeLeadTime rdf:type owl:Class ;
                rdfs:subClassOf <http://field33.com/ontologies/@fld33/methodology/Metric> ;
                rdfs:comment "One of the critical DevOps metrics to track is lead time for changes. Not to be confused with cycle time (discussed below), lead time for changes is the length of time between when a code change is committed to the trunk branch and when it is in a deployable state."@en ;
                rdfs:label "Change Lead Time"@en ;
                rdfs:seeAlso "https://www.atlassian.com/devops/frameworks/devops-metrics#:~:text=One%20of%20the%20critical%20DevOps,is%20in%20a%20deployable%20state."@en .


###  http://field33.com/ontologies/@fld33_domain/software_team_metric/CycleTime
:CycleTime rdf:type owl:Class ;
           rdfs:subClassOf <http://field33.com/ontologies/@fld33/methodology/Metric> ;
           rdfs:comment "Cycle time is the time a team spends working on an item until it is ready for shipment. In the development world, cycle time is the time from when developers make a commit to the moment its deployed to production."@en ;
           rdfs:label "Cycle Time"@en ;
           rdfs:seeAlso "https://www.atlassian.com/devops/frameworks/devops-metrics#:~:text=One%20of%20the%20critical%20DevOps,is%20in%20a%20deployable%20state."@en .


###  http://field33.com/ontologies/@fld33_domain/software_team_metric/DeploymentFrequency
:DeploymentFrequency rdf:type owl:Class ;
                     rdfs:subClassOf <http://field33.com/ontologies/@fld33/methodology/Metric> ;
                     rdfs:comment "Understanding the frequency of how often new code is deployed into production is critical to understanding DevOps success. Many practitioners use the term delivery to mean code changes that are released into a pre-production staging environment, and reserve deployment to refer to code changes that are released into production."@en ;
                     rdfs:label "Deployment Frequency"@en ;
                     rdfs:seeAlso "https://www.atlassian.com/devops/frameworks/devops-metrics#:~:text=One%20of%20the%20critical%20DevOps,is%20in%20a%20deployable%20state."@en .


###  http://field33.com/ontologies/@fld33_domain/software_team_metric/ErrorDetectionRatio
:ErrorDetectionRatio rdf:type owl:Class ;
                     rdfs:subClassOf <http://field33.com/ontologies/@fld33/methodology/Metric> ;
                     rdfs:label "Error Detection Ratio"@en .


###  http://field33.com/ontologies/@fld33_domain/software_team_metric/ExternalInternalErrorDetectionRatio
:ExternalInternalErrorDetectionRatio rdf:type owl:Class ;
                                     rdfs:subClassOf :ErrorDetectionRatio ;
                                     rdfs:label "External vs. Internal Error Detection Ratio"@en .


###  http://field33.com/ontologies/@fld33_domain/software_team_metric/MTTBF
:MTTBF rdf:type owl:Class ;
       owl:equivalentClass :MeanTimeToBugFix ;
       rdfs:subClassOf <http://field33.com/ontologies/@fld33/methodology/Metric> ;
       rdfs:label "MTTBF"@en .


###  http://field33.com/ontologies/@fld33_domain/software_team_metric/MTTF
:MTTF rdf:type owl:Class ;
      owl:equivalentClass :MeanTimeToFailure ;
      rdfs:subClassOf <http://field33.com/ontologies/@fld33/methodology/Metric> ;
      rdfs:label "MTTF"@en .


###  http://field33.com/ontologies/@fld33_domain/software_team_metric/MTTR
:MTTR rdf:type owl:Class ;
      owl:equivalentClass :MeanTimeToRecovery ;
      rdfs:subClassOf <http://field33.com/ontologies/@fld33/methodology/Metric> ;
      rdfs:label "MTTR"@en .


###  http://field33.com/ontologies/@fld33_domain/software_team_metric/MeanTimeToBugFix
:MeanTimeToBugFix rdf:type owl:Class ;
                  rdfs:subClassOf <http://field33.com/ontologies/@fld33/methodology/Metric> ;
                  rdfs:comment "Mean Time To Bug Fix is the average time it takes someone to fix the registered defect. To calculate that metric, you should be tracking following fields in your bug tracker: defect registration date and time."@en ;
                  rdfs:label "Mean Time To Bug Fix"@en ;
                  rdfs:seeAlso "https://www.atlassian.com/incident-management/kpis/common-metrics"@en .


###  http://field33.com/ontologies/@fld33_domain/software_team_metric/MeanTimeToFailure
:MeanTimeToFailure rdf:type owl:Class ;
                   rdfs:subClassOf <http://field33.com/ontologies/@fld33/methodology/Metric> ;
                   rdfs:comment "Mean time to failure (MTTF) is a maintenance metric that measures the average amount of time a non-repairable asset operates before it fails. Because MTTF is relevant only for assets and equipment that cannot or should not be repaired, MTTF can also be thought of as the average lifespan of an asset."@en ;
                   rdfs:label "Mean Time To Failure"@en ;
                   rdfs:seeAlso "https://www.fiixsoftware.com/maintenance-metrics/mean-time-to-failure/#:~:text=Mean%20time%20to%20failure%20(MTTF)%20is%20a%20maintenance%20metric%20that,average%20lifespan%20of%20an%20asset."@en .


###  http://field33.com/ontologies/@fld33_domain/software_team_metric/MeanTimeToRecovery
:MeanTimeToRecovery rdf:type owl:Class ;
                    rdfs:subClassOf <http://field33.com/ontologies/@fld33/methodology/Metric> ;
                    rdfs:comment "Mean time to recovery (MTTR) measures how long it takes to recover from a partial service interruption or total failure. This is an important metric to track, regardless of whether the interruption is the result of a recent deployment or an isolated system failure."@en ;
                    rdfs:label "Mean Time To Recovery"@en ;
                    rdfs:seeAlso "https://www.atlassian.com/devops/frameworks/devops-metrics#:~:text=One%20of%20the%20critical%20DevOps,is%20in%20a%20deployable%20state."@en .


###  http://field33.com/ontologies/@fld33_domain/software_team_metric/PsychologicalSafety
:PsychologicalSafety rdf:type owl:Class ;
                     rdfs:subClassOf <http://field33.com/ontologies/@fld33/methodology/Metric> ;
                     rdfs:comment "Psychological safety is being able to show and employ ones self without fear of negative consequences of self image, status or career (Kahn 1990, p. 708). It can be defined as a shared belief that the team is safe for interpersonal risk taking. In psychologically safe teams, team members feel accepted and respected."@en ;
                     rdfs:label "Psychological Safety"@en ;
                     rdfs:seeAlso "https://en.wikipedia.org/wiki/Psychological_safety"@en .


###  http://field33.com/ontologies/@fld33_domain/software_team_metric/WaitingTime
:WaitingTime rdf:type owl:Class ;
             rdfs:subClassOf <http://field33.com/ontologies/@fld33/methodology/Metric> ;
             rdfs:label "Waiting Time"@en .


###  Generated by the OWL API (version 4.5.9.2019-02-01T07:24:44Z) https://github.com/owlcs/owlapi
